Changed the semantics to cover external rq/rs correctly

src/Prototype/Correctness.v
@@ -1,12 +1,58 @@
 Require Import Bool List String Peano_dec Eqdep.
-Require Import FnMap Language SingleValue Transaction.
+Require Import FnMap Language SingleValue Transaction Simulation.
+Require Import FunctionalExtensionality.
 
 Section System.
   Variables extIdx1 extIdx2: nat.
 
-  Theorem impl_linear: Linear (impl extIdx1 extIdx2).
+  Local Definition IState := State SingleValueMsg ImplState.
+  Local Definition SState := State SingleValueMsg SpecState.
+
+  Definition validValue (p c1 c2: ImplState) :=
+    match impl_status p with
+    | Valid => Some (impl_value p)
+    | _ => match impl_status c1 with
+           | Valid => Some (impl_value c1)
+           | _ => match impl_status c2 with
+                  | Valid => Some (impl_value c2)
+                  | _ => None
+                  end
+           end
+    end.
+
+  Notation " [ ] " := (@empty _ _).
+  Notation " m [ k <- v ] " := (idx_add k v m) (at level 30).
+
+  Local Definition sim (ist: IState) (sst: SState): Prop.
   Proof.
+    destruct ist as [ioss imsgs].
+    refine (exists iosp iosc1 iosc2,
+               ioss = [][child2Idx <- iosc2][child1Idx <- iosc1][parentIdx <- iosp] /\ _).
+    refine (match validValue iosp iosc1 iosc2 with
+            | Some v => _
+            | None => _
+            end).
+    - exact (sst = {| st_oss := [][specIdx <- v];
+                      st_msgs := imsgs |}).
+    - exact True. (* TODO *)
+  Defined.
+
+  Theorem sim_simulates:
+    Simulates sim (impl extIdx1 extIdx2) (spec extIdx1 extIdx2).
+  Proof.
+    unfold Simulates; intros.
+    
   Admitted.
+
+  Theorem impl_refines_spec:
+    Refines (impl extIdx1 extIdx2) (spec extIdx1 extIdx2).
+  Proof.
+    apply simulation_implies_refinement with (sim:= sim).
+    - apply sim_simulates.
+    - do 3 eexists; split; reflexivity.
+  Qed.
+
+  (* Theorem impl_linear: Linear (impl extIdx1 extIdx2). *)
 
 End System.
 
